fc_evval beginning

coq/stlc3.v
@@ -305,14 +305,74 @@ Proof.
   Case "VAbs".
     repeat constructor. destruct s; try solve by inversion.
     simpl in H11. inversion H11; subst.
+    Admitted.
 
+Lemma index_fc: forall H x v,
+   fc_env H ->
+   index x H = Some v ->
+   fc_val v.
+Proof.
+   intros.
+   induction H0.
+     inversion H1.
+     case_eq (beq_nat x (length vheap)); intros E; simpl in H1.
+     + rewrite E in H1. inversion H1; subst. eauto.
+     + rewrite E in H1. eauto.
+Qed.
+
+Definition get_fenv (vs : option (option vl_stack)) :=
+  match vs with
+  | Some (Some (vabs_stack h _ _ _)) => h
+  | _ => []
+  end.
 
 Theorem fc_eval : forall k fr lS env_stack t v_stack,
   teval_stack k (fr::lS) env_stack t First = v_stack ->
+  fc_env env_stack ->
   fc v_stack.
 Proof.
-admit.
-Qed.
+  intros.
+  destruct v_stack as [v_stack|].
+  destruct v_stack as [v_stack|].
+  generalize dependent fr. generalize dependent lS. generalize dependent env_stack0.
+  generalize dependent t. generalize dependent v_stack.
+  induction k; intros.
+  Case "k = 0". inversion H.
+  Case "k = S k". destruct t;[SCase "True"|SCase "False"|SCase "Var"|SCase "App"|SCase "Abs"]; inversion H; subst.
+       
+     SCase "True". constructor. constructor.
+     SCase "False". constructor. constructor.
+   
+     - SCase "Var". destruct v; try solve by inversion.
+       rewrite H2. constructor. eapply index_fc. eassumption. inversion H2. eauto.
+  
+     - SCase "App".
+       
+       remember (fr::lS) as lS1.
+       remember (teval_stack k lS1 env_stack0 t1 Second) as tf_stack.
+
+       destruct tf_stack as [tf_stack|]; try solve by inversion.
+       destruct tf_stack as [tf_stack|]; try solve by inversion.
+       destruct tf_stack; try solve by inversion.
+ 
+       remember (teval_stack k lS1 env_stack0 t2 c) as tx_stack.
+       
+       destruct tx_stack as [tx_stack|]; try solve by inversion.
+       destruct tx_stack as [tx_stack|]; try solve by inversion.
+
+       remember (get_stack_frame lS1 s) as frame.
+       
+       destruct frame; try solve by inversion. destruct p.
+       destruct c; simpl in H2. simpl.
+
+       destruct s.
+       
+       eapply IHk with (env_stack0 := (vbool_stack b :: h)).
+       econstructor. eapply IHk; eauto. rewrite Heqtx_stack. subst lS1. eauto.
+
+       
+ 
+       
 
 Theorem teval_equiv : forall k n t env v lS fr env_stack v_stack,
      teval k env t n = v ->
@@ -400,315 +460,3 @@ Proof.
           eapply equiv_abs. simpl.
           assert (beq_nat (length lS) (length lS) = true) as A. eapply beq_nat_true_iff. eauto. rewrite A. eauto. eauto. 
 Qed.
-
-
-(* TODO: 
-
-Theorem: The lifetimes of second-class values follow a stack discipline.
-
-We define a lower-level operational
-semantics that splits environments into first-class and second-class parts,
-and maintains a stack of second-class environments through all
-function calls. Closures will contain a first-class environment but
-only a stack pointer to represent the second-class part. When invoking
-a closure, the stack pointer will be used to find the correct caller
-environment in which to resolve the callee's free second-class variables.
-Proving equivalence of the high-level and low-level semantics will
-establish this proposition.
-
-Tentative rules:
-
-N,M ::= nat
-H,S ::= 0 | H,x:v
-
-
-H S_0,..,S_N |- c ⇓^n c    CST
-
-x^m:v  in  H S_N^[<=n]
------------------------    VAR
-H S0,..,SN |- x^m ⇓^n v
-
-H S0,..,SN |- λx^m.t ⇓^n  <H N, λx^m.t>    ABS
-
-H S0,..,SM,..,SN |- t1 ⇓^2  <H' M, λx^m.t3>
-H S0,..,SM,..,SN |- t2 ⇓^m  v2
-H S0,..,SM,..,SN,(SM x^m: v2) |- t3 ⇓^1  v3
--------------------------------------------    APP
-H S0,..,SM,..,SN |- t1 t2 ⇓^n v3
-
-
-We want to prove that this semantics is equivalent to teval above.
-
-How to do this we need to define alternative version (_stack) of
-the following:
-
-  Inductive vl_stack : Type      (because closures are different here)
-
-  Definition venv_stack          (this will be a pair (list vl) * (list list vl),
-                                  the H S0,..,SN above)
-
-  Fixpoint teval_stack(k: nat)(env: venv_stack)(t: tm)(n: class){struct k}: option (option vl_stack) :=
-
-And then have correspondences that relate vl/vl_stack, venv/venv_stack, etc.
-Let's call these corr_vl, corr_venv, ... .
-
-The final theorem we want to prove is:
-
-  Theorem eval_equiv : forall n e c G GS v vS,
-    corr_venv G GS ->
-    teval n G e c = v -> 
-    teval_stack n GS c = vS ->
-    corr_vl v vS.
-
-So, given corresponding environments, the two eval functions produce a
-corresponding result.
-
-*)
-
-
-
-
-
-
-Hint Constructors ty.
-Hint Constructors tm.
-Hint Constructors vl.
-
-
-Hint Constructors has_type.
-Hint Constructors val_type.
-Hint Constructors wf_env.
-
-Hint Constructors option.
-Hint Constructors list.
-Hint Constructors env.
-
-Hint Unfold index.
-Hint Unfold length.
-Hint Unfold expand_env.
-
-Hint Resolve ex_intro.
-
-Definition length_env {X : Type} (c : class) (env : env X): nat :=
-match env, c with
-| Def l1 l2 n, First => length l1
-| Def l1 l2 n, Second => length l2
-end
-.
-
-Hint Unfold expand_env.
-
-Lemma length_env_incr : forall (X : Type) n m env (x : X),
-   n = m ->
-   length_env n (expand_env env x m) = 1 + length_env n env.
-Proof.
-  intros. destruct env; destruct n; inversion H; auto.
-Qed.
-   
-Lemma length_env_same : forall (X : Type) n m env (x : X),
-   n <> m ->
-   length_env n (expand_env env x m) = length_env n env.
-Proof.
-  intros. destruct env0; destruct n; destruct m.
-      apply ex_falso_quodlibet; auto.
-      auto.
-      auto.
-      apply ex_falso_quodlibet; auto.
-Qed.
-
-Hint Rewrite length_env_incr.
-Hint Rewrite length_env_same.
-Hint Unfold not.
-
-Lemma wf_length : forall vs ts,
-      wf_env vs ts ->
-      length_env First vs = length_env First ts /\ length_env Second vs = length_env Second ts.
-Proof.
-  intros. induction H. auto.
-  destruct IHwf_env.
-  destruct n. 
-  Case "First"; split.
-  repeat rewrite length_env_incr; auto.
-  repeat rewrite length_env_same; auto.
-  unfold not; intros. inversion H3. unfold not; intros. inversion H3.
-  Case "Second"; split.
-  repeat rewrite length_env_same; auto.
-  unfold not; intros. inversion H3. unfold not; intros. inversion H3.
-  repeat rewrite length_env_incr; auto.
-Qed.
-
-Hint Immediate wf_length.
-
-Definition get_class (x : var): class :=
-match x with
-| VFst _ => First
-| VSnd _ => Second
-end
-.
-
-Definition get_idx (x : var): nat :=
-match x with
-| VFst n => n
-| VSnd n => n
-end
-.
-
-Lemma index_max : forall X vs x (T: X),
-                       lookup x vs = Some T ->
-                       get_idx x < length_env (get_class x) vs.
-Proof.
-  intros X vs; destruct vs as [l1 l2 n].
-  intros x T H.
-  destruct x; simpl.
-  Case "VFst"; induction l1.
-    SCase "nil". intros. inversion H.
-    SCase "cons".
-       intros. inversion H.
-       case_eq (beq_nat i (length l1)); intros E.
-       SSCase "hit".
-          rewrite E in H1. inversion H1. subst.
-          eapply beq_nat_true in E. 
-          unfold length. unfold length in E. rewrite E. eauto.
-       SSCase "miss".
-          rewrite E in H1.
-          assert (i < length l1). eapply IHl1. apply H1.
-          compute. eauto.
-  Case "VSnd"; induction l2.
-    SCase "nil". inversion H. destruct (ble_nat i n); inversion H1.
-    SCase "cons". intros. inversion H.
-       case_eq (beq_nat i (length l2)); intros E.
-       SSCase "hit".
-          rewrite E in H1. inversion H1. subst.
-          eapply beq_nat_true in E. 
-          unfold length. unfold length in E. rewrite E. eauto.
-       SSCase "miss".
-          rewrite E in H1.
-          assert (i < length l2). eapply IHl2. apply H1.
-          compute. eauto.
-Qed.
-
-Lemma valtp_extend : forall vs v v1 T,
-                       val_type vs v T ->
-                       val_type (v1::vs) v T.
-Proof. intros. induction H; eauto. Qed.
-
-Lemma index_extend : forall X vs n a (T: X),
-                       index n vs = Some T ->
-                       index n (a::vs) = Some T.
-
-Proof.
-  intros.
-  assert (n < length vs). eapply index_max. eauto.
-  assert (n <> length vs). omega.
-  assert (beq_nat n (length vs) = false) as E. eapply beq_nat_false_iff; eauto.
-  unfold index. unfold index in H. rewrite H. rewrite E. reflexivity.
-Qed.
-
-
-Lemma index_safe_ex: forall H1 G1 TF i,
-             wf_env H1 G1 ->
-             index i G1 = Some TF ->
-             exists v, index i H1 = Some v /\ val_type H1 v TF.
-Proof. intros. induction H.
-       Case "nil". inversion H0.
-       Case "cons". inversion H0.
-         case_eq (beq_nat i (length ts)).
-           SCase "hit".
-             intros E.
-             rewrite E in H3. inversion H3. subst t.
-             assert (beq_nat i (length vs) = true). eauto.
-             assert (index i (v :: vs) = Some v). eauto.  unfold index. rewrite H2. eauto.
-             eauto.
-           SCase "miss".
-             intros E.
-             assert (beq_nat i (length vs) = false). eauto.
-             rewrite E in H3.
-             assert (exists v0, index i vs = Some v0 /\ val_type vs v0 TF) as HI. eapply IHwf_env. eauto.
-           inversion HI as [v0 HI1]. inversion HI1. 
-           eexists. econstructor. eapply index_extend; eauto. eapply valtp_extend; eauto.
-Qed.
-
-  
-Inductive res_type: venv -> option vl -> ty -> Prop :=
-| not_stuck: forall venv v T,
-      val_type venv v T ->
-      res_type venv (Some v) T.
-
-Hint Constructors res_type.
-Hint Resolve not_stuck.
-
-
-Lemma valtp_widen: forall vf H1 H2 T1 T2,
-  val_type H1 vf T1 ->
-  stp H1 T1 H2 T2 ->
-  val_type H2 vf T2.
-Proof.
-  intros. inversion H; inversion H0; subst T2; subst; eauto.
-Qed.
-
-
-Lemma invert_abs: forall venv vf vx T1 T2,
-  val_type venv vf (TFun T1 T2) ->
-  exists env tenv y T3 T4,
-    vf = (vabs env y) /\ 
-    wf_env env tenv /\
-    has_type (T3::(TFun T3 T4)::tenv) y T4 /\
-    stp venv T1 (vx::vf::env) T3 /\
-    stp (vx::vf::env) T4 venv T2.
-Proof.
-  intros. inversion H. repeat eexists; repeat eauto.
-Qed.
-
-
-(* if not a timeout, then result not stuck and well-typed *)
-
-Theorem full_safety : forall n e tenv venv res T,
-  teval n venv e = Some res -> has_type tenv e T -> wf_env venv tenv ->
-  res_type venv res T.
-
-Proof.
-  intros n. induction n.
-  (* 0 *)   intros. inversion H.
-  (* S n *) intros. destruct e; inversion H; inversion H0.
-  
-  Case "True".  eapply not_stuck. eapply v_bool.
-  Case "False". eapply not_stuck. eapply v_bool.
-
-  Case "Var".
-    destruct (index_safe_ex venv0 tenv0 T i) as [v [I V]]; eauto. 
-
-    rewrite I. eapply not_stuck. eapply V.
-
-  Case "App".
-    remember (teval n venv0 e1) as tf.
-    remember (teval n venv0 e2) as tx. 
-    subst T.
-    
-    destruct tx as [rx|]; try solve by inversion.
-    assert (res_type venv0 rx T1) as HRX. SCase "HRX". subst. eapply IHn; eauto.
-    inversion HRX as [? vx]. 
-
-    destruct tf as [rf|]; subst rx; try solve by inversion.  
-    assert (res_type venv0 rf (TFun T1 T2)) as HRF. SCase "HRF". subst. eapply IHn; eauto.
-    inversion HRF as [? vf].
-
-    destruct (invert_abs venv0 vf vx T1 T2) as
-        [env1 [tenv [y0 [T3 [T4 [EF [WF [HTY [STX STY]]]]]]]]]. eauto.
-    (* now we know it's a closure, and we have has_type evidence *)
-
-    assert (res_type (vx::vf::env1) res T4) as HRY.
-      SCase "HRY".
-        subst. eapply IHn. eauto. eauto.
-        (* wf_env f x *) econstructor. eapply valtp_widen; eauto.
-        (* wf_env f   *) econstructor. eapply v_abs; eauto.
-        eauto.
-
-    inversion HRY as [? vy].
-
-    eapply not_stuck. eapply valtp_widen; eauto.
-    
-  Case "Abs". intros. inversion H. inversion H0.
-    eapply not_stuck. eapply v_abs; eauto.
-Qed.
-
-End STLC2.
